<rdf:RDF xmlns:rdf="http://www.w3.org/1999/02/22-rdf-syntax-ns#" xmlns:rdfs="http://www.w3.org/2000/01/rdf-schema#" xmlns:daml="http://www.daml.org/2001/03/daml+oil#" xmlns:sumo="http://reliant.teknowledge.com/DAML/SUMO.daml#" xmlns="http://reliant.teknowledge.com/DAML/terroristAttackTypes.daml#">
  <!--  copyright 2003 (c) Teknowledge 						-->
  <!--  This program is free software; you can redistribute it and/or		-->
  <!--  modify it under the terms of the GNU Lesser General Public		-->
  <!--  License as published by the Free Software Foundation; either		-->
  <!--  version 2.1 of the License, or (at your option) any later version.	-->
  <!--										-->
  <!--  This program is distributed in the hope that it will be useful,		-->
  <!--  but WITHOUT ANY WARRANTY; without even the implied warranty of		-->
  <!--  MERCHANTABILITY or FITNESS FOR A PARTICULAR PURPOSE.  See the GNU		-->
  <!--  Lesser General Public License for more details.				-->
  <!--										-->
  <!--  You should have received a copy of the GNU Lesser General Public		-->
  <!--  License along with this program; if not, write to the Free Software	-->
  <!--  Foundation, Inc., 59 Temple Place, Suite 330, Boston, MA 02111-1307 USA	-->
  <rdfs:Class rdf:ID="Arson">
    <rdfs:subClassOf rdf:resource="http://reliant.teknowledge.com/DAML/SUMO.daml#Combustion" />
    <rdfs:subClassOf rdf:resource="http://reliant.teknowledge.com/DAML/SUMO.daml#Destruction" />
    <rdfs:comment>
      An act where an agent sets something which it does not possess
      on fire in order to destroy it or its contents.
    </rdfs:comment>
  </rdfs:Class>
  <rdfs:Class rdf:ID="Bomb">
    <rdfs:subClassOf rdf:resource="http://reliant.teknowledge.com/DAML/SUMO.daml#Weapon" />
    <rdfs:comment>A weapon that explodes in order to cause damage.</rdfs:comment>
  </rdfs:Class>
  <rdfs:Class rdf:ID="Bombing">
    <rdfs:subClassOf rdf:resource="http://reliant.teknowledge.com/DAML/SUMO.daml#Destruction" />
    <rdfs:comment>
      An act of Destruction where the thing destroyed
      is destroyed by means of an explosive device.
    </rdfs:comment>
  </rdfs:Class>
  <rdfs:Class rdf:ID="Bus">
    <rdfs:subClassOf rdf:resource="#Vehicle" />
    <rdfs:comment>
      An automobile designed to carry at least
      a dozen people.  It can be distinguished from a van which is
      designed to carry less than a dozen people.
    </rdfs:comment>
  </rdfs:Class>
  <rdfs:Class rdf:ID="BusStop">
    <rdfs:subClassOf rdf:resource="http://reliant.teknowledge.com/DAML/SUMO.daml#GeographicArea" />
    <rdfs:comment>
      An area, often, though not necessarily with
      seats or some kind of minimal shelter, where people gather to meet and
      board a bus.  It must border a road.
    </rdfs:comment>
  </rdfs:Class>
  <rdfs:Class rdf:ID="BusinessPerson">
    <rdfs:subClassOf rdf:resource="http://reliant.teknowledge.com/DAML/SUMO.daml#OccupationalRole" />
    <rdfs:comment>
      Any of a class of people in a professional
      occupation such as banking, finance, management, or engineering.  This is
      distinguished from blue collar jobs that primarily involve manual labor
      rather than thought as the effort expended to derive remuneration.  It is
      also distinguished from professions that may be outwardly similar but are
      done in a non-profit organization.
    </rdfs:comment>
  </rdfs:Class>
  <rdfs:Class rdf:ID="CarBombing">
    <rdfs:subClassOf rdf:resource="#Bombing" />
    <rdfs:comment>
      A car bombing is an attack in which a car is
      used as the delivery mechanism for a bomb.  The car is usually destroyed
      in the blast if the bomb detonates successfully.
    </rdfs:comment>
  </rdfs:Class>
  <rdfs:Class rdf:ID="CargoVehicle">
    <rdfs:subClassOf rdf:resource="#Vehicle" />
    <rdfs:comment>
      Any vehicle that is designed to move things
      other than humans as its primary purpose.  It is distinguished from buses
      and troop carriers that are designed to move people.
    </rdfs:comment>
  </rdfs:Class>
  <rdfs:Class rdf:ID="Celebrity">
    <rdfs:subClassOf rdf:resource="http://reliant.teknowledge.com/DAML/SUMO.daml#Human" />
    <rdfs:comment>
      Anyone who is known by a large number of people,
      either explicitly by name, or by action.
    </rdfs:comment>
  </rdfs:Class>
  <rdfs:Class rdf:ID="Checkpoint">
    <rdfs:subClassOf rdf:resource="http://reliant.teknowledge.com/DAML/SUMO.daml#GeographicArea" />
    <rdfs:comment>
      An area on or very near a border, usually along
      a road connecting two regions, where MilitaryPersons or Police
      restrict the flow of traffic in order to extract tarrifs, deny movement to
      certain kinds of people or goods, or other enforement actions.  Because of
      the power relationship involved, such areas are often the site of illegal
      activities conducted by the officials in order to extract favors or
      bribes.
    </rdfs:comment>
  </rdfs:Class>
  <rdfs:Class rdf:ID="ChemicalAttack">
    <rdfs:subClassOf rdf:resource="http://reliant.teknowledge.com/DAML/SUMO.daml#ViolentContest" />
    <rdfs:comment>
      An attack against people or property in which
      a chemical agent is used as the active ingredient of the attack.
    </rdfs:comment>
  </rdfs:Class>
  <rdfs:Class rdf:ID="Civilian">
    <rdfs:subClassOf rdf:resource="http://reliant.teknowledge.com/DAML/SUMO.daml#OccupationalRole" />
    <rdfs:comment>
      Someone who is not a member of a
      ModernMilitaryOrganization.
    </rdfs:comment>
  </rdfs:Class>
  <rdfs:Class rdf:ID="CivilianHuman">
    <rdfs:subClassOf rdf:resource="http://reliant.teknowledge.com/DAML/SUMO.daml#Human" />
    <rdfs:comment>
      A Human who is not a member of a
      ModernMilitaryOrganization.
    </rdfs:comment>
  </rdfs:Class>
  <rdfs:Class rdf:ID="Convoy">
    <rdfs:subClassOf rdf:resource="http://reliant.teknowledge.com/DAML/SUMO.daml#Group" />
    <rdfs:comment>
      A group of people driving vehicles that all have
      the same destination.  That destination may be an intermediate destination
      on the way to a final destination for some of the vehicles however.  This
      is distinguished from vehicles that have no common purpose, such as
      traffic on a freeway.  This includes cases where some of the agents intend
      to reach a point but fail to do so.
    </rdfs:comment>
  </rdfs:Class>
  <rdfs:Class rdf:ID="Diplomat">
    <rdfs:subClassOf rdf:resource="#GovernmentPerson" />
    <rdfs:comment>
      A person who works as a facilitator for communication
      between countries, in the official employ of one of the countries.
    </rdfs:comment>
  </rdfs:Class>
  <rdfs:Class rdf:ID="Dissident">
    <rdfs:subClassOf rdf:resource="#Civilian" />
    <rdfs:comment>
      Someone who is opposed to the leadership
      of a particular country.  Typically, a dissident suffers punishment
      at the hands of the country whose leadership he is opposing.
    </rdfs:comment>
  </rdfs:Class>
  <rdfs:Class rdf:ID="EducationalFacility">
    <rdfs:subClassOf rdf:resource="http://reliant.teknowledge.com/DAML/SUMO.daml#StationaryArtifact" />
    <rdfs:comment>
      A building or campus, owned by an
      EducationalOrganization, which is intended as the location for
      EducationalProcesses.
    </rdfs:comment>
  </rdfs:Class>
  <rdfs:Class rdf:ID="Embassy">
    <rdfs:subClassOf rdf:resource="#GovernmentBuilding" />
    <rdfs:comment>
      An embassy is a building that is owned by a
      government to house its diplomatic and consular staff that is in
      another country.
    </rdfs:comment>
  </rdfs:Class>
  <rdfs:Class rdf:ID="EntertainmentBuilding">
    <rdfs:subClassOf rdf:resource="http://reliant.teknowledge.com/DAML/SUMO.daml#Building" />
    <rdfs:comment>
      A building that has the primary
      purpose of entertaining people.
    </rdfs:comment>
  </rdfs:Class>
  <rdfs:Class rdf:ID="Factory">
    <rdfs:subClassOf rdf:resource="http://reliant.teknowledge.com/DAML/SUMO.daml#Building" />
    <rdfs:comment>
      A building intended to house a process that
      produces goods of some value.
    </rdfs:comment>
  </rdfs:Class>
  <rdfs:Class rdf:ID="Garage">
    <rdfs:subClassOf rdf:resource="http://reliant.teknowledge.com/DAML/SUMO.daml#Building" />
    <rdfs:comment>
      A building, the intended function of which is to
      contain and protect vehicles when they are not in use or are under
      repair.
    </rdfs:comment>
  </rdfs:Class>
  <rdfs:Class rdf:ID="GovernmentBuilding">
    <rdfs:subClassOf rdf:resource="http://reliant.teknowledge.com/DAML/SUMO.daml#Building" />
    <rdfs:comment>A building belonging to a Government</rdfs:comment>
  </rdfs:Class>
  <rdfs:Class rdf:ID="GovernmentPerson">
    <rdfs:subClassOf rdf:resource="http://reliant.teknowledge.com/DAML/SUMO.daml#OccupationalRole" />
    <rdfs:comment>A person who works for a Government.</rdfs:comment>
  </rdfs:Class>
  <rdfs:Class rdf:ID="HandGrenade">
    <rdfs:subClassOf rdf:resource="#Bomb" />
    <rdfs:comment>
      A hand grenade is a small explosive device
      with a simple trigger mechanism, usually lasting a few seconds, designed
      to be propelled by a human to its target.
    </rdfs:comment>
  </rdfs:Class>
  <rdfs:Class rdf:ID="HandgrenadeAttack">
    <rdfs:subClassOf rdf:resource="#Bombing" />
    <rdfs:comment>
      An attack in which a HandGrenade is
      employed as an explosive device for the purpose of Destruction.
      A case in which a hand grenade is used as a blunt striking object in
      an attack would not be in this class.
    </rdfs:comment>
  </rdfs:Class>
  <rdfs:Class rdf:ID="Hijacking">
    <rdfs:subClassOf rdf:resource="http://reliant.teknowledge.com/DAML/SUMO.daml#UnilateralGetting" />
    <rdfs:comment>
      An event in which a TransportationDevice is
      taken by coercion or force by an agent.
    </rdfs:comment>
  </rdfs:Class>
  <rdfs:Class rdf:ID="HostageTaking">
    <rdfs:subClassOf rdf:resource="http://reliant.teknowledge.com/DAML/SUMO.daml#UnilateralGetting" />
    <rdfs:comment>
      An event in which one agent keeps another
      against his or her will, in order to force it or a third agent to
      accede to some demand.  The hostages are typically kept in the place
      where they are first taken hostage, in contrast to a Kidnapping.
      Hostage taking often involves a number of people (although it may be
      just one), again, in contrast to a Kidnapping.
    </rdfs:comment>
  </rdfs:Class>
  <rdfs:Class rdf:ID="Hotel">
    <rdfs:subClassOf rdf:resource="http://reliant.teknowledge.com/DAML/SUMO.daml#Building" />
    <rdfs:comment>
      A building which servers the purpose of a temporary
      home for people, either for people who are travelling, or occasionally for
      those who do not have another more permanent residence.  A hotel is
      distinguished from a homeless shelter, or a residence loaned to a friend
      in that the primary purpose of the building is to generate revenue in
      return for the priviledge of staying there.  Many hotels contains other
      facilities such as restaurants or health clubs or even miscellaneous stores
      although that is not their primary business or purpose.
    </rdfs:comment>
  </rdfs:Class>
  <rdfs:Class rdf:ID="IncendiaryDeviceAttack">
    <rdfs:subClassOf rdf:resource="http://reliant.teknowledge.com/DAML/SUMO.daml#Combustion" />
    <rdfs:subClassOf rdf:resource="http://reliant.teknowledge.com/DAML/SUMO.daml#ViolentContest" />
    <rdfs:comment>
      An attack in which an agent
      uses a device which causes fire in order to destroy life or property.
    </rdfs:comment>
  </rdfs:Class>
  <rdfs:Class rdf:ID="Infiltration">
    <rdfs:subClassOf rdf:resource="http://reliant.teknowledge.com/DAML/SUMO.daml#JoiningAnOrganization" />
    <rdfs:comment>
      An event in which an agent joins an
      organization under false pretenses.  The objective of such an act
      is often to gather information helpful to a rival organization.
    </rdfs:comment>
  </rdfs:Class>
  <rdfs:Class rdf:ID="Kidnapping">
    <rdfs:subClassOf rdf:resource="http://reliant.teknowledge.com/DAML/SUMO.daml#UnilateralGetting" />
    <rdfs:comment>
      An event in which one agent keeps another
      against his or her will, in order to force it or a third agent to
      accede to some demand.  The kidnapped party is normally removed from
      the location where first attacked.  In contrast to a HotageTaking,
      a kidnapping normally involves an attack on one, or a very small
      number of people, such as a couple.
    </rdfs:comment>
  </rdfs:Class>
  <rdfs:Class rdf:ID="Knife">
    <rdfs:subClassOf rdf:resource="http://reliant.teknowledge.com/DAML/SUMO.daml#Device" />
    <rdfs:comment>
      A sharp object used for cutting.  The object must
      have at least single blade or major protrusion which may be sharp at its
      end as well.  It may be sharp on both sides, or just one.  Unlike an awl
      it has a sharp edge rather than a point.  Unlike scissors, it is a single
      blade without additional articulated parts.  Unlike an axe, a knife is
      well-designed for slicing rather than chopping, although a heavy knife
      such as a broadsword can also be used for chopping, whereas a non-knife is
      not well designed for slicing meat for example.  A knife can be small like
      a pocket knife, or large like a two-handed broadsword.  A knife may also
      include other protrusions such as in the split swords and trident-like
      objects (that also possess a long sharp edge) in Chinese weaponry.
    </rdfs:comment>
  </rdfs:Class>
  <rdfs:Class rdf:ID="KnifeAttack">
    <rdfs:subClassOf rdf:resource="http://reliant.teknowledge.com/DAML/SUMO.daml#ViolentContest" />
    <rdfs:comment>An attack in which a knife is used.</rdfs:comment>
  </rdfs:Class>
  <rdfs:Class rdf:ID="LandVehicle">
    <rdfs:subClassOf rdf:resource="#Vehicle" />
    <rdfs:comment>A Vehicle designed to move on land.</rdfs:comment>
  </rdfs:Class>
  <rdfs:Class rdf:ID="LetterBombAttack">
    <rdfs:subClassOf rdf:resource="#Bombing" />
    <rdfs:comment>
      An attack with a bomb that is
      concealed in a letter or package, which is typically designed to
      explode upon opening.
    </rdfs:comment>
  </rdfs:Class>
  <rdfs:Class rdf:ID="Lynching">
    <rdfs:subClassOf rdf:resource="http://reliant.teknowledge.com/DAML/SUMO.daml#Killing" />
    <rdfs:comment>
      A lynching is a form of Killing conducted under
      a thin guise of legitimacy by a vigilante group.  It may be a purge of an
      individual from the group who is perceived to have gone astray, or it may
      be the summary execution of an individual outside the group that the group
      has determined has violated some law or code, either of the group, or the
      larger society.  A lynching is distinguished from a legal execution in
      that the laws of a government are not followed in carrying out the
      killing.  A lynching is distinguished from a murder in that there is the
      pretense of some process carried out by a group in the name of their own
      group or a higher power.
    </rdfs:comment>
  </rdfs:Class>
  <rdfs:Class rdf:ID="Marketplace">
    <rdfs:subClassOf rdf:resource="http://reliant.teknowledge.com/DAML/SUMO.daml#GeographicArea" />
    <rdfs:comment>
      An area, building, or set of buildings
      where FinancialTransactions are intended to take place.  There should
      be more than one owner or renter of space or buildings within the
      marketplace.
    </rdfs:comment>
  </rdfs:Class>
  <rdfs:Class rdf:ID="Militant">
    <rdfs:subClassOf rdf:resource="#Civilian" />
    <rdfs:comment>
      A militant is a civilian who is not
      officially authorized by a government to engage in combat, but who
      does so on behalf of a PoliticalOrganization.
    </rdfs:comment>
  </rdfs:Class>
  <rdfs:Class rdf:ID="MilitaryOrganization">
    <rdfs:subClassOf rdf:resource="#NationalGovernment" />
    <rdfs:comment>
      Any heavily armed Organization
      that is part of a Government and that is charged with representing the
      Government in international conflicts.
    </rdfs:comment>
  </rdfs:Class>
  <rdfs:Class rdf:ID="MilitaryPerson">
    <rdfs:subClassOf rdf:resource="http://reliant.teknowledge.com/DAML/SUMO.daml#OccupationalRole" />
    <rdfs:comment>
      Someone who is a member of a
      ModernMilitaryOrganization.
    </rdfs:comment>
  </rdfs:Class>
  <rdfs:Class rdf:ID="ModernMilitaryOrganization">
    <rdfs:subClassOf rdf:resource="#MilitaryOrganization" />
    <rdfs:comment>
      A subclass of
      MilitaryOrganization. An instance of ModernMilitaryOrganization is a
      military organization of current (or recent) times, having modern equipment
      and methods. Generally includes organizations making at least some use of
      high-tech military technology.
    </rdfs:comment>
  </rdfs:Class>
  <rdfs:Class rdf:ID="Mortar">
    <rdfs:subClassOf rdf:resource="http://reliant.teknowledge.com/DAML/SUMO.daml#Weapon" />
    <rdfs:comment>
      A mortar is a bomb that is shot at a location.  A
      howitzer is a weapon that fires mortars.  The mortar may not include the
      propelling charge that provides the motive force for delivering it to its
      target, which distinguishes it from a rocket.  A mortar is distinguished
      from other bombs in that it is propelled rather than exploded in place, or
      dropped, or propelled by human power.
    </rdfs:comment>
  </rdfs:Class>
  <rdfs:Class rdf:ID="MortarAttack">
    <rdfs:subClassOf rdf:resource="#Bombing" />
    <rdfs:comment>
      An attack in which a Mortar weapon is
      used.
    </rdfs:comment>
  </rdfs:Class>
  <rdfs:Class rdf:ID="NationalGovernment">
    <rdfs:subClassOf rdf:resource="http://reliant.teknowledge.com/DAML/SUMO.daml#Government" />
    <rdfs:comment>
      The class of Governments whose
      jurisdictions are Nations.
    </rdfs:comment>
  </rdfs:Class>
  <rdfs:Class rdf:ID="OfficeBuilding">
    <rdfs:subClassOf rdf:resource="http://reliant.teknowledge.com/DAML/SUMO.daml#Building" />
    <rdfs:comment>
      A building in which work activities take
      place which is not primarily designed for manufacturing or retail sales.
    </rdfs:comment>
  </rdfs:Class>
  <rdfs:Class rdf:ID="PeaceKeepingMission">
    <rdfs:subClassOf rdf:resource="#ModernMilitaryOrganization" />
    <rdfs:comment>
      A military deployment which is intended
      to prevent hostilities between two other entities located in the same rough
      geographic area.
    </rdfs:comment>
  </rdfs:Class>
  <rdfs:Class rdf:ID="PlaceOfWorship">
    <rdfs:subClassOf rdf:resource="http://reliant.teknowledge.com/DAML/SUMO.daml#Building" />
    <rdfs:comment>Any place designed for ReligiousProcesses.</rdfs:comment>
  </rdfs:Class>
  <rdfs:Class rdf:ID="PoliceFacility">
    <rdfs:subClassOf rdf:resource="http://reliant.teknowledge.com/DAML/SUMO.daml#Building" />
    <rdfs:comment>A building designed to house PolicePersons.</rdfs:comment>
  </rdfs:Class>
  <rdfs:Class rdf:ID="PolicePerson">
    <rdfs:subClassOf rdf:resource="#GovernmentPerson" />
    <rdfs:comment>
      A member of a government whose occupation
      has the primary purpose of preventing crime and arresting criminals.
    </rdfs:comment>
  </rdfs:Class>
  <rdfs:Class rdf:ID="PoliticalFigure">
    <rdfs:subClassOf rdf:resource="#Celebrity" />
    <rdfs:comment>
      A well known person who participates
      in a PoliticalProcess.  This must either be the person's principal
      occupation, or what is intended to become his principal occupation
      (for example, after an election).
    </rdfs:comment>
  </rdfs:Class>
  <rdfs:Class rdf:ID="ReligiousFigure">
    <rdfs:subClassOf rdf:resource="#Celebrity" />
    <rdfs:comment>A well-known leader of a religious group.</rdfs:comment>
  </rdfs:Class>
  <rdfs:Class rdf:ID="Restaurant">
    <rdfs:subClassOf rdf:resource="http://reliant.teknowledge.com/DAML/SUMO.daml#Building" />
    <rdfs:comment>
      A building where people pay to be served food
      and eat.  Some restaurants may also offer entertainment.
    </rdfs:comment>
  </rdfs:Class>
  <rdfs:Class rdf:ID="Road">
    <rdfs:subClassOf rdf:resource="http://reliant.teknowledge.com/DAML/SUMO.daml#Region" />
    <rdfs:comment>
      A path along which vehicles travel.  It is typically,
      although not necessarily, paved and intended for cars.
    </rdfs:comment>
  </rdfs:Class>
  <rdfs:Class rdf:ID="Rocket">
    <rdfs:subClassOf rdf:resource="http://reliant.teknowledge.com/DAML/SUMO.daml#Weapon" />
  </rdfs:Class>
  <rdfs:Class rdf:ID="RocketMissileAttack">
    <rdfs:subClassOf rdf:resource="#Bombing" />
    <rdfs:comment>
      An attack in which a rocket or
      missile is used.
    </rdfs:comment>
  </rdfs:Class>
  <rdfs:Class rdf:ID="Stoning">
    <rdfs:subClassOf rdf:resource="http://reliant.teknowledge.com/DAML/SUMO.daml#ViolentContest" />
    <rdfs:comment>
      An act where a victim or victims is attacked
      with stones.  The stones may either be placed on top of a victim in
      order to cause death by pressure and suffocation, in which case the act
      is typically part of a ritualized legal sentence, or where the victim
      is pelted with stones causing injury or death by trauma.  The intent
      of such an act is usually the death of the victim.
    </rdfs:comment>
  </rdfs:Class>
  <rdfs:Class rdf:ID="Store">
    <rdfs:subClassOf rdf:resource="http://reliant.teknowledge.com/DAML/SUMO.daml#Building" />
    <rdfs:comment>
      A Building that has the purpose of housing
      FinancialTransactions.
    </rdfs:comment>
  </rdfs:Class>
  <rdfs:Class rdf:ID="StoreOwner">
    <rdfs:subClassOf rdf:resource="http://reliant.teknowledge.com/DAML/SUMO.daml#OccupationalRole" />
    <rdfs:comment>
      Someone who operates a store which he
      either owns or rents.
    </rdfs:comment>
  </rdfs:Class>
  <rdfs:Class rdf:ID="Student">
    <rdfs:subClassOf rdf:resource="http://reliant.teknowledge.com/DAML/SUMO.daml#SocialRole" />
    <rdfs:comment>
      A person who participates in an
      EducationalProcess in order to learn something.
    </rdfs:comment>
  </rdfs:Class>
  <rdfs:Class rdf:ID="Subway">
    <rdfs:subClassOf rdf:resource="http://reliant.teknowledge.com/DAML/SUMO.daml#Hole" />
    <rdfs:comment>
      A subway is a hollow area of the earth, typically
      under large cities, designed for running trains that move people. It is
      distinguished from other kinds of tunnels in that trains run through
      them, primarily for the purpose of carrying people rather than ore, for
      example.
    </rdfs:comment>
  </rdfs:Class>
  <rdfs:Class rdf:ID="SuicideBombing">
    <rdfs:subClassOf rdf:resource="#Bombing" />
    <rdfs:subClassOf rdf:resource="http://reliant.teknowledge.com/DAML/SUMO.daml#Killing" />
    <rdfs:comment>
      A bomb attack in which the bomber
      intends to blow himself up during the course of the attack.  The bomber
      is the delivery mechanism for the explosive and the bomb is typically
      in close contact with the bomber, such as being strapped around his
      torso.  This action is distinguished from actions in which the bomber
      merely happens to be blown up by his own bomb in that the bomber
      knows that he is committing suicide.
    </rdfs:comment>
  </rdfs:Class>
  <rdfs:Class rdf:ID="Tourist">
    <rdfs:subClassOf rdf:resource="http://reliant.teknowledge.com/DAML/SUMO.daml#SocialRole" />
    <rdfs:comment>
      A tourist is a person who is travelling to a
      place primarily for reasons of entertainment or education, rather than
      business, although business transaction may take place during the trip.
    </rdfs:comment>
  </rdfs:Class>
  <rdfs:Class rdf:ID="TouristSite">
    <rdfs:subClassOf rdf:resource="http://reliant.teknowledge.com/DAML/SUMO.daml#GeographicArea" />
    <rdfs:comment>
      A tourist site is a location that has some
      feature of interest to Tourists, which entertains or informs them.
    </rdfs:comment>
  </rdfs:Class>
  <rdfs:Class rdf:ID="Vandalism">
    <rdfs:subClassOf rdf:resource="http://reliant.teknowledge.com/DAML/SUMO.daml#Destruction" />
    <rdfs:comment>
      An event where the objective of the agent
      is to damage or destroy some property of another agent.  This is
      distinguished from acts where the prime objective is damage or loss
      of life of another agent.
    </rdfs:comment>
  </rdfs:Class>
  <rdfs:Class rdf:ID="Vehicle"></rdfs:Class>
  <rdfs:Class rdf:ID="VehicleAttack">
    <rdfs:subClassOf rdf:resource="http://reliant.teknowledge.com/DAML/SUMO.daml#ViolentContest" />
    <rdfs:comment>
      An event in which a vehicle is used
      by an agent in order to inflict injury, death or damage to people
      or property.
    </rdfs:comment>
  </rdfs:Class>
  <daml:DatatypeProperty rdf:ID="agentCountInAttack">
    <rdfs:comment>
      (agentCountInAttack ?ACT ?COUNT)
      means that in the Destruction event ?ACT, the number of agents involved
      was a NonNegativeInteger, ?COUNT.
    </rdfs:comment>
    <rdf:type rdf:resource="http://reliant.teknowledge.com/DAML/SUMO.daml#BinaryPredicate" />
    <rdfs:domain rdf:resource="http://reliant.teknowledge.com/DAML/SUMO.daml#Destruction" />
    <rdfs:range rdf:resource="http://reliant.teknowledge.com/DAML/SUMO.daml#NonNegativeInteger" />
  </daml:DatatypeProperty>
  <daml:DatatypeProperty rdf:ID="dayOfEvent">
    <rdfs:comment>
      (dayOfEvent ?EVENT ?N) means that the ?EVENT
      of Process type happened at the ?N-th day of the month, where ?N is of
      PositiveInteger type.
    </rdfs:comment>
    <rdf:type rdf:resource="http://reliant.teknowledge.com/DAML/SUMO.daml#BinaryPredicate" />
    <rdfs:domain rdf:resource="http://reliant.teknowledge.com/DAML/SUMO.daml#Process" />
    <rdfs:range rdf:resource="http://reliant.teknowledge.com/DAML/SUMO.daml#PositiveInteger" />
  </daml:DatatypeProperty>
  <daml:ObjectProperty rdf:ID="monthOfEvent">
    <rdfs:comment>
      (monthOfEvent ?EVENT ?MONTH) means that the
      ?EVENT of Process type happened at the ?MONTH of the year, where ?MONTH
      is of Month type.
    </rdfs:comment>
    <rdf:type rdf:resource="http://reliant.teknowledge.com/DAML/SUMO.daml#BinaryPredicate" />
    <rdfs:domain rdf:resource="http://reliant.teknowledge.com/DAML/SUMO.daml#Process" />
    <rdfs:range rdf:resource="http://reliant.teknowledge.com/DAML/SUMO.daml#Month" />
  </daml:ObjectProperty>
  <daml:ObjectProperty rdf:ID="targetTypeInAttack">
    <rdfs:comment>
      (targetTypeInAttack ?ACT ?TYPE) means
      that in the Destruction event ?ACT, the target was an Object of type
      ?TYPE.
    </rdfs:comment>
    <rdf:type rdf:resource="http://reliant.teknowledge.com/DAML/SUMO.daml#BinaryPredicate" />
    <rdfs:domain rdf:resource="http://reliant.teknowledge.com/DAML/SUMO.daml#Destruction" />
    <rdfs:range rdf:resource="http://reliant.teknowledge.com/DAML/SUMO.daml#Object" />
  </daml:ObjectProperty>
  <daml:DatatypeProperty rdf:ID="victimCasualtyCount">
    <rdfs:comment>
      (victimCasualtyCount ?ACT ?COUNT)
      means that in the Destruction event ?ACT, the total number of victims
      killed and injured was a NonNegativeInteger,?COUNT.
    </rdfs:comment>
    <rdf:type rdf:resource="http://reliant.teknowledge.com/DAML/SUMO.daml#BinaryPredicate" />
    <rdfs:domain rdf:resource="http://reliant.teknowledge.com/DAML/SUMO.daml#Destruction" />
    <rdfs:range rdf:resource="http://reliant.teknowledge.com/DAML/SUMO.daml#NonNegativeInteger" />
  </daml:DatatypeProperty>
  <daml:DatatypeProperty rdf:ID="victimDeathCount">
    <rdfs:comment>
      (victimDeathCount ?ACT ?COUNT) means
      that in the Destruction event ?ACT, the number of victims who died was a
      NonNegativeInteger, ?COUNT.
    </rdfs:comment>
    <rdf:type rdf:resource="http://reliant.teknowledge.com/DAML/SUMO.daml#BinaryPredicate" />
    <rdfs:domain rdf:resource="http://reliant.teknowledge.com/DAML/SUMO.daml#Destruction" />
    <rdfs:range rdf:resource="http://reliant.teknowledge.com/DAML/SUMO.daml#NonNegativeInteger" />
  </daml:DatatypeProperty>
  <daml:DatatypeProperty rdf:ID="victimInjuryCount">
    <rdfs:comment>
      (victimInjuryCount ?ACT ?COUNT) means
      that in the Destruction event ?ACT, the number of victim injured was a
      NonNegativeInteger, ?COUNT.
    </rdfs:comment>
    <rdf:type rdf:resource="http://reliant.teknowledge.com/DAML/SUMO.daml#BinaryPredicate" />
    <rdfs:domain rdf:resource="http://reliant.teknowledge.com/DAML/SUMO.daml#Destruction" />
    <rdfs:range rdf:resource="http://reliant.teknowledge.com/DAML/SUMO.daml#NonNegativeInteger" />
  </daml:DatatypeProperty>
  <daml:DatatypeProperty rdf:ID="yearOfEvent">
    <rdfs:comment>
      (yearOfEvent ?EVENT ?N) means that the
      ?EVENT of Process type happened at the ?N-th year,A.D., if ?N is a
      non-negative integer, or at the -?N-th year, B.C., otherwise.
    </rdfs:comment>
    <rdf:type rdf:resource="http://reliant.teknowledge.com/DAML/SUMO.daml#BinaryPredicate" />
    <rdfs:domain rdf:resource="http://reliant.teknowledge.com/DAML/SUMO.daml#Process" />
    <rdfs:range rdf:resource="http://reliant.teknowledge.com/DAML/SUMO.daml#Integer" />
  </daml:DatatypeProperty>
</rdf:RDF>